src/Lean4Lean/ContT.lean
@@ -1,0 +1,61 @@
+def ContT (r : Type u) (m : Type u → Type v) (α : Type w) :=
+  (α → m r) → m r
+
+namespace ContT
+
+variable {r : Type u} {m : Type u → Type v} {α β : Type w}
+
+def run : ContT r m α → (α → m r) → m r :=
+  id
+
+def run' [Monad m] (c : ContT r m r) : m r := do
+  c.run fun x => do pure x
+
+-- TODO why doesn't this work?
+instance [Monad m] : Coe (ContT r m r) (m r) where
+  coe m := m.run'
+
+def map (f : m r → m r) (x : ContT r m α) : ContT r m α :=
+  f ∘ x
+
+theorem run_contT_map_contT (f : m r → m r) (x : ContT r m α) : run (map f x) = f ∘ run x :=
+  rfl
+
+def withContT (f : (β → m r) → α → m r) (x : ContT r m α) : ContT r m β := fun g => x <| f g
+
+theorem run_withContT (f : (β → m r) → α → m r) (x : ContT r m α) :
+    run (withContT f x) = run x ∘ f :=
+  rfl
+
+@[ext]
+protected theorem ext {x y : ContT r m α} (h : ∀ f, x.run f = y.run f) : x = y := by
+  unfold ContT; ext; apply h
+
+instance : Monad (ContT r m) where
+  pure x f := f x
+  bind x f g := x fun i => f i g
+
+instance : LawfulMonad (ContT r m) := LawfulMonad.mk'
+  (id_map := by intros; rfl)
+  (pure_bind := by intros; ext; rfl)
+  (bind_assoc := by intros; ext; rfl)
+
+def monadLift [Monad m] {α} : m α → ContT r m α := fun x f => x >>= f
+
+instance [Monad m] : MonadLift m (ContT r m) where
+  monadLift := ContT.monadLift
+
+theorem monadLift_bind [Monad m] [LawfulMonad m] {α β} (x : m α) (f : α → m β) :
+    (monadLift (x >>= f) : ContT r m β) = monadLift x >>= monadLift ∘ f := by
+  ext
+  simp only [monadLift, MonadLift.monadLift, (· ∘ ·), (· >>= ·), bind_assoc, id, run,
+    ContT.monadLift]
+
+instance (ε) [MonadExcept ε m] : MonadExcept ε (ContT r m) where
+  throw e _ := throw e
+  tryCatch act h f := tryCatch (act f) fun e => h e f
+
+def dud [Monad m] (c : ContT r m r) : ContT T m r := do
+  liftM $ ContT.run' c
+
+end ContT
