src/Lean4Lean/Ext.lean
@@ -1,0 +1,97 @@
+import Lean4Lean.RecM
+
+namespace Lean.TypeChecker.Inner
+
+def toKernelException (m : EIO Exception α) : EIO KernelException (Sum α Exception) := fun x =>
+  match m x with
+  | .ok s I => .ok (.inl s) I
+  | .error e I => .ok (.inr e) I
+
+
+def runMetaM (m : MetaM T) : RecM T := do
+  let mut options := (← readThe Context).options
+  let m' := Lean.Meta.MetaM.run m {lctx := (← readThe Context).lctx, fuel := (← readThe Context).fuel - 1} |>.run {options := options, fileName := default, fileMap := default, maxHeartbeats := 0} {env := (← readThe Context).env'}
+  match ← toKernelException m' with
+  | .inl ((reqs, _), _) => pure reqs
+  | .inr (.internal _ _) => throw $ .other "untranslated Exception.Internal"
+  | .inr (.error _ d) => throw $ .other (← d.toString)
+
+
+open Lean.Meta in
+def extMatch (getT : MetaM (Expr × List Expr)) (localMarker : Name) (lems : List Name) (dbg := false) : RecMO T (Option (Expr × List Expr)) := do
+  if (← readThe Context).fuel == 0 then
+    return none
+  -- options := options.insert `trace.Meta.isDefEq (.ofBool true)
+  -- let localDfEqs := (← readThe Context).localDfEqs
+  -- if dbg then 
+  --   dbg_trace s!"DBG[387]: TypeChecker.lean:406 (after if dbg then)"
+
+  let ret? ← runMetaM (do
+    let mut localLems := []
+    for decl in (← getLCtx) do
+      if dbg then 
+        dbg_trace s!"Checking: {decl.userName} : {← ppExpr decl.type}"
+      if let .app (.const n []) _ := decl.type.getForallBody then -- TODO remove once we can generate lemmas for intermediate reducts
+        if n == localMarker then
+          let newType ← forallTelescope decl.type fun vs b => mkForallFVars vs b.appArg!
+          localLems := localLems ++ [(decl.toExpr, .some newType)]
+          if dbg then 
+            dbg_trace s!"Added: {decl.userName} : {← ppExpr decl.type}"
+
+    let mut candidates := (← lems.mapM (mkConstWithFreshMVarLevels ·)).zip (List.replicate lems.length none)
+    candidates := candidates ++ localLems
+    withLCtx' (← read).lctx do
+      let (T, _) ← getT
+      let condString := do pure s!"{← ppExpr $ ← T.mvarId!.getType}"
+      -- let dbg := (← readThe Core.Context).options.get? `trace.Kernel.ext
+      trace[Kernel.ext] "Trying to show {← condString}"
+      let tryExtEq lem type? T ts := do
+        try
+          trace[Kernel.ext] s!"Trying to apply (fuel {(← read).fuel}): {← ppExpr $ lem} : {← ppExpr $ (← Meta.inferType lem)} to {← condString}"
+          let gs ← T.mvarId!.apply lem (cfg := {shallow := true}) type?
+
+          trace[Kernel.ext] s!"Applying OK:{← ppExpr $ (← Meta.inferType lem)} to  {← condString}\n  {← gs.mapM (do ppExpr $ ← ·.getType)}\n  {← localLems.mapM (do ppExpr $ ← Meta.inferType ·.1)}"
+          if dbg then
+            dbg_trace s!"Applying OK:{← ppExpr $ (← Meta.inferType lem)} to  {← condString}\n  {← gs.mapM (do ppExpr $ ← ·.getType)}\n  {← localLems.mapM (do ppExpr $ ← Meta.inferType ·.1)}"
+          for g in gs do
+            -- TODO unassign T if any g.refl fails?
+            try
+              trace[Kernel.ext] s!"Trying reflection: {← ppExpr $ ← g.getType}"
+              g.refl
+              trace[Kernel.ext] s!"Reflection OK: {← ppExpr $ ← g.getType}"
+            catch e =>
+              trace[Kernel.ext] s!"Reflection FAIL: {← ppExpr $ ← g.getType}"
+              throw e
+          trace[Kernel.ext] s!"Showing OK: {← ppExpr $ ← T.mvarId!.getType}"
+          let TInst ← instantiateMVars T
+          let tsInst ← ts.mapM fun t => instantiateMVars t
+          return some (TInst, tsInst)
+        catch e =>
+          trace[Kernel.ext] s!"Applying FAIL: {← ppExpr $ lem} : {← ppExpr $ (← Meta.inferType lem)} to {← condString}"
+          if dbg then
+            dbg_trace s!"Applying FAIL: {← ppExpr $ lem} : {← ppExpr $ (← Meta.inferType lem)} to {← condString}"
+          pure none
+      for (lem, type?) in candidates do
+        -- for eqMvar in [tEqsMvar, sEqtMvar] do
+        -- TODO is there a way to "undo" assignments from previous failed unification attempts,
+        -- rather than making new mvars every time?
+        let (T, ts) ← getT
+        if let .some prf ← tryExtEq lem type? T ts then
+          printTraces
+          return some prf
+      trace[Kernel.ext] "Showing FAIL: {← ppExpr $ ← T.mvarId!.getType}"
+      printTraces
+      return none
+    )
+
+  if let some (prf, ts) := ret? then
+    if prf.hasExprMVar then
+      throw $ .other "unexpected mvar found in extensional equality proof"
+    if ts.any (·.hasExprMVar) then
+      throw $ .other "unexpected mvar found in extensionally assigned variable"
+    -- check that the proof returned by unification is well-typed with the kernel itself,
+    -- to minimize the trust that we place on unification
+    _ ← inferType prf (inferOnly := false)
+    return some (prf, ts)
+
+  return none
