src/Lean4Lean/RecM.lean
@@ -1,0 +1,96 @@
+import Lean4Lean.Declaration
+import Lean4Lean.Level
+import Lean4Lean.Quot
+import Lean4Lean.Inductive.Reduce
+import Lean4Lean.Instantiate
+import Lean4Lean.ForEachExprV
+import Lean4Lean.EquivManager
+import Lean4Lean.ContT
+import Lean.Meta.Tactic.DfEq
+import Lean.Meta.Tactic.Rewrite
+import Lean.Meta.Tactic.Apply
+import Lean.Meta.Tactic.Replace
+import Lean.Meta.Tactic.Refl
+
+namespace Lean
+
+abbrev InferCache := ExprMap Expr
+
+structure TypeChecker.State where
+  ngen : NameGenerator := { namePrefix := `_kernel_fresh, idx := 0 }
+  inferTypeI : InferCache := {}
+  inferTypeC : InferCache := {}
+  whnfCoreCache : ExprMap Expr := {}
+  whnfCache : ExprMap Expr := {}
+  eqvManager : EquivManager := {}
+  failure : Std.HashSet (Expr × Expr) := {}
+
+structure TypeChecker.Context where
+  env : Kernel.Environment
+  env' : Environment
+  lctx : LocalContext := {}
+  options : Options := default
+  fuel : Nat := 5
+  safety : DefinitionSafety := .safe
+  lparams : List Name := []
+
+namespace TypeChecker
+
+abbrev M := ReaderT Context <| StateT State <| EIO KernelException
+abbrev MO (T : Type) := ContT T M
+
+def M.run (env : Kernel.Environment) (env' : Environment) (safety : DefinitionSafety := .safe) (lctx : LocalContext := {}) (options : Options)
+    (x : M α) (fuel := 5) (localDfEqs : List Expr := []) : EIO KernelException α :=
+  x { env, env', safety, lctx, fuel, options } |>.run' {}
+
+-- instance : MonadEnv M where
+--   getEnv := return (← read).env
+--   modifyEnv _ := pure ()
+
+def getKEnv : M Kernel.Environment := return (← read).env
+
+instance : MonadLCtx M where
+  getLCtx := return (← read).lctx
+
+instance [Monad m] : MonadNameGenerator (StateT State m) where
+  getNGen := return (← get).ngen
+  setNGen ngen := modify fun s => { s with ngen }
+
+instance (priority := low) : MonadWithReaderOf LocalContext M where
+  withReader f := withReader fun s => { s with lctx := f s.lctx }
+
+structure Methods where
+  isDefEqCore : Nat → Expr → Expr → Level → Expr → MO T Bool
+  whnfCore (e : Expr) (l : Option (Level × Expr) := none) (cheapRec := false) (cheapProj := false) : MO T Expr
+  whnf (e : Expr) (d : Option (Level × Expr)) : MO T Expr 
+  inferType (e : Expr) (inferOnly : Bool) : MO T Expr
+
+abbrev RecM := ReaderT Methods M
+abbrev RecMO (T : Type) := ContT T RecM
+abbrev RecMB := ContT Bool RecM
+
+-- TODO can this be derived from a more general rule?
+instance (priority := low) : MonadWithReaderOf LocalContext RecM where
+  withReader f m := fun b c => m b ({c with lctx := f c.lctx})
+
+-- TODO can this be derived from a more general rule?
+instance (priority := low) : MonadWithReaderOf LocalContext (RecMO T) where
+  withReader f m := fun b meths c => m b meths ({c with lctx := f c.lctx})
+
+inductive ReductionStatus where
+  | continue (tn sn : Expr)
+  | unknown (tn sn : Expr)
+  | bool (b : Bool)
+
+namespace Inner
+
+def isDefEqCore (n : Nat) (t s : Expr) (l : Level) (T : Expr) : RecMO U Bool := fun f m => m.isDefEqCore n t s l T (fun a => f a m)
+
+def whnfCore (e : Expr) (l : Option (Level × Expr) := none) (cheapRec := false) (cheapProj := false) : RecMO T Expr :=
+  -- TODO what exactly is going on here?
+  fun f m => m.whnfCore e l cheapRec cheapProj fun e => f e m
+
+
+def whnf (e : Expr) (d : Option (Level × Expr) := none) : RecMO T Expr := fun f m => m.whnf e d fun e => f e m
+
+def inferType (e : Expr) (inferOnly := true) : RecMO T Expr := fun f m => m.inferType e inferOnly fun a => f a m
